QuickSortInLean/Vec.lean
@@ -1,0 +1,72 @@
+import Std.Data.Option.Basic
+import Std.Data.Fin.Basic
+import Std.Data.Array.Lemmas
+
+/--
+When proving termination and the safety of array operation, it's crucial to show
+that each operation preserves the size of the array. Therefore, we encode the
+size into the type using the Vec type.
+-/
+abbrev Vec (α : Type) (n : Nat) := { arr : Array α // arr.size = n }
+
+instance : CoeDep (Array α) arr (Vec α arr.size) where
+  coe := ⟨arr, by rfl⟩
+
+def Vec.get (self : Vec α n) (i : Fin n) : α :=
+  self.val.get ⟨i, by simp [self.property, i.isLt]⟩
+
+instance : GetElem (Vec α n) (Fin n) α (fun _ _ => True) where
+  getElem v i _ := v.get i
+
+instance {α : Type} {n : Nat} : GetElem (Vec α n) Nat α (fun _ i => i < n) where
+  getElem v i isLt := v.get ⟨i, isLt⟩
+
+def Vec.set (self : Vec α n) (i : Fin n) (v : α) : Vec α n :=
+  ⟨self.val.set ⟨i, by simp [self.property, i.isLt]⟩ v, by simp [self.property]⟩
+
+def Vec.swap (self : Vec α n) (i j : Fin n) : Vec α n :=
+  ⟨self.val.swap (i.cast self.property.symm) (j.cast self.property.symm), by simp [self.property]⟩
+
+theorem Vec.get_set_eq (a : Vec α n) (i : Fin n) (v : α) :
+  (a.set i v)[i] = v := by
+  show (a.set i v).get i = v
+  simp [Vec.get, Vec.set]
+
+theorem Vec.get_set_ne (a : Vec α n) (i j : Fin n) (v : α) (h : i ≠ j) :
+  (a.set i v)[j] = a[j] := by
+  show (a.set i v).get j = a.get j
+  simp [Vec.get, Vec.set]
+  exact Array.get_set_ne (j := j.val) a.val ⟨i, by simp [a.property, i.isLt]⟩ v
+    (by simp [a.property, j.isLt]) (Fin.val_ne_of_ne h)
+
+theorem Vec.get_set (a : Vec α n) (i j : Fin n) (v : α) :
+  (a.set i v)[j] = if i = j then v else a[j] := by
+  if h : i = j then
+    simp [h]
+    exact Vec.get_set_eq a j v
+  else
+    simp [h]
+    exact Vec.get_set_ne a i j v h
+
+theorem Vec.swap_def (a : Vec α n) (i j : Fin n) :
+  a.swap i j = (a.set i (a.get j)).set j (a.get i) := by
+  simp [Vec.swap]
+  apply Subtype.eq
+  simp [Vec.get, Vec.set, Array.swap_def]
+  rfl
+
+theorem Vec.get_swap_left {α : Type} {n : Nat} (a : Vec α n) (i j : Fin n) :
+  (a.swap i j)[i] = a[j] := by
+  simp [Vec.swap_def, Vec.get_set, Vec.get_set_eq]
+  cases decEq j i <;> simp [*] <;> rfl
+
+theorem Vec.get_swap_right {α : Type} {n : Nat} (a : Vec α n) (i j : Fin n) :
+  (a.swap i j)[j] = a[i] := by
+  simp [Vec.swap_def, Vec.get_set_eq]
+  rfl
+
+theorem Vec.get_swap_neq {α : Type} {n : Nat} (a : Vec α n) (i j k : Fin n)
+  (ki : k ≠ i) (kj : k ≠ j) :
+  (a.swap i j)[k] = a[k] := by
+  simp [Vec.swap_def]
+  rw [Vec.get_set_ne (h := kj.symm), Vec.get_set_ne (h := ki.symm)]
